code/k256/Hacl.K256.Scalar.fsti
@@ -10,7 +10,9 @@ open Lib.Buffer
 module ST = FStar.HyperStack.ST
 module LSeq = Lib.Sequence
 module BSeq = Lib.ByteSequence
+
 module S = Spec.K256
+module SG = Hacl.Spec.K256.GLV
 
 module BD = Hacl.Bignum.Definitions
 
@@ -164,3 +166,13 @@ val is_qelem_le_q_halved_vartime: f:qelem -> Stack bool
   (requires fun h -> live h f)
   (ensures  fun h0 b h1 -> modifies0 h0 h1 /\
     b == (qas_nat h0 f <= S.q / 2))
+
+
+val qmul_shift_384 (res a b: qelem) : Stack unit
+  (requires fun h ->
+    live h a /\ live h b /\ live h res /\
+    eq_or_disjoint a b /\ eq_or_disjoint a res /\ eq_or_disjoint b res /\
+    qas_nat h a < S.q /\ qas_nat h b < S.q)
+  (ensures  fun h0 _ h1 -> modifies (loc res) h0 h1 /\
+    qas_nat h1 res < S.q /\
+    qas_nat h1 res == SG.qmul_shift_384 (qas_nat h0 a) (qas_nat h0 b))
